BigStep.v
@@ -1,5 +1,6 @@
 Require Import SystemFR.Trees.
 Require Import SystemFR.Syntax.
+Require Import SystemFR.RewriteTactics.
 
 Reserved Notation "t '~~>*' v" (at level 20).
 
@@ -11,7 +12,7 @@ Inductive bcbv_step: tree -> tree -> Prop :=
   | BSzero : zero ~~>* zero
 
   (* lambda *)
-  | BSlambda : forall t, 
+  | BSlambda : forall t, 
       notype_lambda t ~~>* notype_lambda t 
   | BSapp : forall t1 b1 t2 v2 v,
       t1 ~~>* notype_lambda b1 ->
@@ -20,3 +21,21 @@ Inductive bcbv_step: tree -> tree -> Prop :=
         app t1 t2 ~~>* v
 where "t '~~>*' v" := (bcbv_step t v).
 
+Hint Constructors bcbv_step : bcbv_step.
+
+Lemma bs_closed_term: forall t1 t2, t1 ~~>* t2 -> closed_term t1 -> closed_term t2.
+Proof.
+  induction 1; repeat light || apply_any; t_closer.
+Qed.
+
+Lemma bs_value: forall t v, t ~~>* v -> cbv_value v.
+Proof.
+  induction 1; repeat light; auto with values.
+Qed.
+
+Lemma value_bs: forall v, cbv_value v -> v ~~>* v .
+Proof.
+  induction 1.
+Admitted.
+
+Hint Immediate bs_value value_bs : values.
